

9/17/25

Last Time

$A = m \times p$ matrix

$B = p \times n$ matrix

"
 $[\vec{b}_1, \dots, \vec{b}_n]$

$$AB = [A\vec{b}_1, \dots, A\vec{b}_n]$$

Example:

$$\begin{bmatrix} 2 & 1 \\ 5 & 3 \end{bmatrix} \begin{bmatrix} 3 & -1 \\ -5 & 2 \end{bmatrix} = \begin{bmatrix} 1 & 0 \\ 0 & 1 \end{bmatrix}$$

Theorem:

If $R: \mathbb{R}^p \rightarrow \mathbb{R}^m$, $S: \mathbb{R}^n \rightarrow \mathbb{R}^p$ are linear transformations then

$R \circ S$ is linear and $[R \circ S] = [R][S]$

$AB \quad A \quad B$

OTOH $(R \circ S)(\vec{x}) = (AB)(\vec{x})$

OTOH $R(S(\vec{x})) = R(B\vec{x}) = A(B\vec{x})$

so $(AB)(\vec{x}) = A(B\vec{x})$

e.g. Why is $AI = A$?

proof 1: Let $R(\vec{y}) = A\vec{y}$, $\text{id}(\vec{x}) = \vec{x}$

then $[R \circ \text{id}] = [R][\text{id}] = AI$

and $R \circ \text{id} = R(\vec{x})$

So $[R \circ \text{id}] = [R] = A$

i.e. $A = AI$

proof 2:

$$\begin{aligned} A I &= A [\vec{e}_1, \dots, \vec{e}_n] \\ &= [A \vec{e}_1, \dots, A \vec{e}_n] \\ &= \begin{bmatrix} \text{1st col of } A & \dots & \text{n}^{\text{th}} \text{ col of } A \end{bmatrix} = A \end{aligned}$$

e.g. $A \cdot (B + C) = A \cdot ([\vec{b}_1, \dots, \vec{b}_n] + [\vec{c}_1, \dots, \vec{c}_n])$ write B+C column wise

$$= A [\vec{b}_1 + \vec{c}_1, \dots, \vec{b}_n + \vec{c}_n]$$
definition of matrix addition
$$= [A(\vec{b}_1 + \vec{c}_1) \dots A(\vec{b}_n + \vec{c}_n)]$$
definition of matrix multiplication
$$= [A\vec{b}_1 + A\vec{c}_1, \dots, A\vec{b}_n + A\vec{c}_n]$$
distributive Law for matrix times vector
$$= [A\vec{b}_1, \dots, A\vec{b}_n] + [A\vec{c}_1, \dots, A\vec{c}_n]$$
definition of matrix addition
$$= A[\vec{b}_1, \dots, \vec{b}_n] + A[\vec{c}_1, \dots, \vec{c}_n]$$
definition of matrix multiplication
$$= AB + AC$$

Prop - Matrix multiplication is associative

Let: A be $m \times p$ matrix,

B be $p \times l$ matrix,

C be $l \times n$ matrix

then $AB(C) = A(BC)$

Let $T(\vec{x}) = C\vec{x}$, $S(\vec{y}) = B\vec{y}$, $R(\vec{z}) = A\vec{z}$

Then - $(R \circ S) \circ T(\vec{x}) = (R \circ S)(T(\vec{x})) = R(S(T(\vec{x})))$

OTOH:

$R \circ (S \circ T)(\vec{x}) = R(S \circ T(\vec{x})) = R(S(T(\vec{x})))$

So

$$R \circ (S \circ T) = (R \circ S) \circ T$$

$$\rightarrow [R \circ (S \circ T)] = [(R \circ S) \circ T]$$

$$\rightarrow [R][S \circ T] = [R \circ S][T]$$

$$\rightarrow [R]([S][T]) = ([R][S])[T]$$

$$\rightarrow A(BC) = (AB)C$$

